theories/case_studies/lse_downward/lse_adequacy.v
@@ -574,10 +574,6 @@ Section Adequacy.
       + solve_addr+H0 H1 H2.
       + solve_addr+H3 H4.
     }
-    iAssert (ot_switcher_prop W0' C LSE_f') as "#ot_switcher_LSE_f_borrow".
-    { replace LSE_f' with (borrow (WSealable LSE_f)) by (subst LSE_f LSE_f'; done).
-      by iApply ot_switcher_prop_borrow.
-    }
 
     assert (ot_switcher ∉ dom (seal_std W0)) as Hot_notin_W0.
     { by subst W0. }
@@ -587,14 +583,8 @@ Section Adequacy.
       as "(Hseals_C & Hsts_C & Hseal_LSE_f)"; first done.
     { iIntros (w); iApply mono_priv_ot_switcher. }
     { subst W0'.
-      destruct (decide (WSealable LSE_f = LSE_f')) as [Heq_sb|Heq_sb].
-        - rewrite -Heq_sb.
-          replace {[WSealable LSE_f; WSealable LSE_f]} with ({[WSealable LSE_f]} : gset Word) by set_solver+.
-          rewrite big_sepS_singleton.
-          done.
-        - rewrite big_sepS_insert; last set_solver+.
-          rewrite big_sepS_singleton.
-          iSplitL; done.
+      rewrite normalise_sealed_words_borrow.
+      rewrite big_sepS_singleton; iFrame "ot_switcher_LSE_f".
     }
     subst W0'; set (W0' := <o[ ot_switcher := {[ WSealable LSE_f; LSE_f' ]}]o> W0).
 
@@ -649,7 +639,6 @@ Section Adequacy.
         rewrite C_exp_tbl in H2.
         solve_addr+H1 H2.
       }
-      iDestruct (ot_switcher_prop_borrow with "ot_switcher_C_f") as "ot_switcher_C_f'".
 
       assert ( Winter = <o[ot_switcher:=exported_entries_words C_cmpt]o>Wpre ) as HWinter.
       { rewrite /Winter /Wpre /std_update_compartment Hexported_entries_words; done. }
@@ -660,9 +649,8 @@ Section Adequacy.
         as "(Hseals_C & Hsts_C & #Hseal_switcher)".
       { iIntros (w); iApply mono_priv_ot_switcher. }
       { rewrite -HWinter Hexported_entries_words.
-        rewrite -big_sepS_later; iNext.
-        iEval (rewrite union_comm_L); iApply big_sepS_insert_2; first (iFrame "ot_switcher_C_f'").
-        iApply big_sepS_singleton; iFrame "ot_switcher_C_f".
+        rewrite normalise_sealed_words_borrow.
+        rewrite big_sepS_singleton; iFrame "ot_switcher_C_f".
       }
       rewrite -HWinter.
       iFrame.
